wip, exposing full substitutiosn

src/reflection/FStar.Reflection.Basic.fst
@@ -999,10 +999,10 @@ let compare_string s1 s2 = Z.of_int_fs (String.compare s1 s2)
 let push_binder e b = Env.push_binders e [b]
 let push_namedv e b = Env.push_binders e [S.mk_binder b]
 
-let subst (x:bv) (n:term) (m:term) : term =
-  SS.subst [NT(x,n)] m
-
 let close_term (b:binder) (t:term) : term = SS.close [b] t
+
+let subst (s : list subst_elt) (t : term) : term =
+  SS.subst s t
 
 let range_of_term (t:term) = t.pos
 let range_of_sigelt (s:sigelt) = s.sigrng
