ulib/FStar.Reflection.Data.fsti
@@ -23,6 +23,15 @@ let ppname_t = FStar.Sealed.Inhabited.sealed ""
 let as_ppname (x:string) : ppname_t = FStar.Sealed.Inhabited.seal x
 
 noeq
+type subst_elt =
+  | DB : int -> namedv -> subst_elt
+  | NM : namedv -> int -> subst_elt
+  | NT : namedv -> term -> subst_elt
+  | UN : int -> universe -> subst_elt
+  | UD : univ_name -> int -> subst_elt
+type subst = list subst_elt
+
+noeq
 type vconst =
   | C_Unit      : vconst
   | C_Int       : int -> vconst // Not exposing the full details of our integer repr.
